src/program_proof/pb/ghost_proof.v
@@ -1,10 +1,19 @@
 From Perennial.program_proof Require Import grove_prelude.
 
-Section definitions.
 Record pb_names :=
   {
   commit_gn:gname
   }.
+
+Definition Log := list u8.
+
+Definition log_po (lhs rhs:Log) : Prop :=
+  prefix lhs rhs.
+
+Notation "lhs ⪯ rhs" := (log_po lhs rhs)
+(at level 20, format "lhs ⪯ rhs") : bi_scope.
+
+Section definitions.
 
 Context `{!gooseGlobalGS Σ}.
 
@@ -13,7 +22,15 @@ Implicit Type γ : pb_names.
 Definition config_ptsto γ (cn:u64) (conf:list u64): iProp Σ.
 Admitted.
 
-Definition Log := list u8.
+Definition proposal_ptsto γ (cn:u64) (l:Log): iProp Σ.
+Admitted.
+
+Definition proposal_lb γ (cn:u64) (l:Log): iProp Σ.
+Admitted.
+
+(* Probably not needed *)
+Definition proposal_ptsto_ro γ (cn:u64) (l:Log): iProp Σ.
+Admitted.
 
 Definition accepted_ptsto γ (cn:u64) (r:u64) (l:Log): iProp Σ.
 Admitted.
@@ -27,35 +44,22 @@ Admitted.
 Definition commit_ptsto γ (l:Log): iProp Σ.
 Admitted.
 
-Context {γ}.
+Definition accepted_by γ cn l : iProp Σ :=
+  ∃ conf, config_ptsto γ cn conf ∗
+      ∀ (r:u64), ⌜r ∈ conf⌝ → accepted_lb γ cn r l.
 
-Notation "'config(' cn ')↦□' conf" := (config_ptsto γ cn conf)
-(at level 20, format "config( cn )↦□ conf") : bi_scope.
-
-Notation "'accepted(' r ',' cn ')↦□' l" := (accepted_ptsto_ro γ cn r l)
-(at level 20, format "accepted( r , cn )↦□ l") : bi_scope.
-
-Notation "'accepted(' r ',' cn ')≥' l" := (accepted_lb γ cn r l)
-(at level 20, format "accepted( r , cn )≥ l") : bi_scope.
-
-Notation "'proposal(' cn ')≥' l" := (accepted_lb γ cn 0 l)
-(at level 20, format "proposal( cn )≥ l") : bi_scope.
-
-Notation "'commit↦' l" := (commit_ptsto γ l)
-(at level 20, format "commit↦ l") : bi_scope.
+(* oldconfmax *)
+Definition φ γ (cn:u64) log : iProp Σ :=
+  ∀ cn_old log_old ,
+   ⌜int.Z cn_old < int.Z cn⌝ →
+   accepted_by γ cn_old log_old → ⌜log_old ⪯ log⌝.
 
 (* System-wide invariant for primary/backup replication with many replicas with
    configuration changes *)
-Definition pb_invariant : iProp Σ :=
-  ∃ cn_latest l_committed,
-  "Hconfig" ∷ (∀ cn' conf, ⌜cn' < cn_latest⌝ → config(cn')↦□ conf -∗ ∃ r l, ⌜r ∈ conf⌝ ∗
-               accepted(r,cn')↦□ l ∗ proposal(cn_latest)≥ l
-              ) ∗
-  "Hcommit" ∷ commit↦ l_committed ∗
-  "Hprop" ∷ proposal(cn_latest)≥ l_committed ∗
-  "Haccepted" ∷ (∃ cn' conf,
-      (degen(cn_latest) ∨ nondegen(cn_latest) ∗ ⌜cn' = cn_latest⌝) ∗
-      config(cn')↦□ conf ∗ (∀ r, ⌜r ∈ conf⌝ → accepted(r,cn')≥ l_committed))
+Definition pb_invariant γ : iProp Σ :=
+  ∃ cn_committed l_committed,
+  "Hcommit" ∷ commit_ptsto γ l_committed ∗
+  "Haccepted" ∷ accepted_by γ cn_committed l_committed ∗ φ γ cn_committed l_committed
 .
 
 End definitions.
